LeanSubst/Basic.lean
@@ -1,240 +1,186 @@
 
-import LeanSubst.Notation
-import LeanSubst.Monad
-
 namespace LeanSubst
   universe u
-  variable {T : Type u} {F : Type u -> Type u}
+  variable {T : Type}
 
-  namespace Sequence
-    @[simp]
-    def cons {T} (x : T) (xs : Nat -> T) : Nat -> T
-    | 0 => x
-    | n + 1 => xs n
-  end Sequence
+  @[simp]
+  def Sequence.cons {T : Type u} (x : T) (xs : Nat -> T) : Nat -> T
+  | 0 => x
+  | n + 1 => xs n
 
   infixr:55 "::" => Sequence.cons
 
-  def Ren := Nat -> Nat
+  abbrev Ren := Nat -> Nat
 
-  def Subst.Lift (X : Type u) (F : Type u -> Type u) := (Nat -> F X) -> Nat -> F X
+  inductive Subst.Kind : Type where
+  | re | su
 
-  def Subst (T : Type u) (F : Type u -> Type u) := Nat -> F T
+  inductive Subst.Action (T : Type) where
+  | re : Nat -> Subst.Action T
+  | su : T -> Subst.Action T
 
-  class SubstMap (T : Type u) (F : Type u -> Type u) where
-    smap : Subst.Lift T F -> (Nat -> F T) -> T -> T
+  abbrev Subst (T : Type) := Nat -> Subst.Action T
 
-  class HasVar (T : Type u) where
-    to : Nat -> T
-    fro : T -> Nat
-    to_fro_id : ∀ x, fro (to x) = x
+  def SplitSubst (T : Type) : Subst.Kind -> Type
+  | .re => Ren
+  | .su => Subst T
 
-  @[simp]
-  theorem has_var_to_fro_id {T} [HasVar T] {x} : HasVar.fro (HasVar.to (T := T) x) = x := by
-    rw [HasVar.to_fro_id]
+  abbrev Subst.Lift (T : Type) k := SplitSubst T k -> SplitSubst T k
 
-  class ActionOps (T : Type u) (F : Type u -> Type u) [Monad F] where
-    fro : F T -> T
-    to_fro_id : ∀ x, fro (pure x) = x
-
-  @[simp]
-  theorem action_ops_to_fro_id {T F} [Monad F] [ActionOps T F] {x} : ActionOps.fro (T := T) (F := F) (pure x) = x := by
-    rw [ActionOps.to_fro_id]
-
-  class SubstMapVar (T : Type u) (F : Type u -> Type u) [HasVar T] [Monad F] [SubstMap T F] [ActionOps T F] where
-    smap_var {lf f x} : pure (SubstMap.smap (F := F) lf f (HasVar.to (T := T) x)) = f x
-
-  @[simp]
-  theorem subst_map_var {T F} [HasVar T] [Monad F] [SubstMap T F] [ActionOps T F] [SubstMapVar T F] {lf f x}
-    : pure (SubstMap.smap (F := F) lf f (HasVar.to (T := T) x)) = f x
-  := by rw [SubstMapVar.smap_var]
-
-  @[simp]
-  instance instHasVar_ActionF [Monad F] [HasVar T] [ActionOps T F] : HasVar (F T) where
-    to n := pure $ HasVar.to n
-    fro t := HasVar.fro $ ActionOps.fro t
-    to_fro_id := by {
-      intro x
-      rw [ActionOps.to_fro_id]
-      rw [HasVar.to_fro_id]
-    }
-
-  @[simp]
-  instance instActionOps_ActionF [Monad F] [LawfulMonad F] [ActionOps T F] : ActionOps (F T) F where
-    fro := join
-    to_fro_id := by intro x; simp
-
-  @[simp]
-  instance instSubstMap_ActionF [Monad F] [ActionOps T F] [SubstMap T F] : SubstMap (F T) F where
-    smap lf f := Functor.map (SubstMap.smap (F := F) (λ f n => join (lf (λ n => pure (f n)) n)) (join ∘ f))
-
-  variable [HasVar T] [Monad F] [ActionOps T F]
+  class SubstMap (T : Type) where
+    smap : (k : Subst.Kind) -> Subst.Lift T k -> SplitSubst T k -> T -> T
 
   section
-    variable [LawfulMonad F] [SubstMap T F]
+    variable [SubstMap T]
 
     open SubstMap
 
-    namespace Ren
-      def to : Ren -> Subst T F
-      | r, n => HasVar.to (r n)
+    @[coe]
+    def Ren.to : Ren -> Subst T
+    | r => λ n => .re (r n)
 
-      def fro : Subst T F -> Ren
-      | σ, n => HasVar.fro (σ n)
+    @[simp]
+    instance instCoe_Ren_Subst {T} : Coe Ren (Subst T) where
+      coe := Ren.to
 
-      def lift : Ren -> Ren
-      | _, 0 => 0
-      | σ, n + 1 => σ n + 1
+    def Ren.lift : Ren -> Ren
+    | _, 0 => 0
+    | σ, n + 1 => σ n + 1
 
-      def apply (r : Ren) : T -> T := smap (F := F) (to ∘ lift ∘ fro) (to r)
-    end Ren
+    def Ren.apply (r : Ren) : T -> T := smap .re lift r
 
-    namespace Subst
-      def lift : Subst T F -> Subst T F
-      | _, 0 => HasVar.to 0
-      | σ, n + 1 => Ren.apply (F := F) (· + 1) (σ n)
+    def Subst.lift : Subst T -> Subst T
+    | _, 0 => .re 0
+    | σ, n + 1 => match (σ n) with
+      | .su t => .su (Ren.apply (λ n => n + 1) t)
+      | .re k => .re (k + 1)
 
-      def apply (σ : Subst T F) : T -> T := smap lift σ
+    def Subst.apply (σ : Subst T) : T -> T := smap .su lift σ
 
-      def compose : Subst T F -> Subst T F -> Subst T F
-      | σ, τ, n => apply (λ n => pure (f := F) (τ n)) (σ n)
-    end Subst
+    def Subst.compose : Subst T -> Subst T -> Subst T
+    | σ, τ, n => match (σ n) with
+      | .su t => .su (apply τ t)
+      | .re k => τ k
   end
 
-  def I : Subst T F := HasVar.to
-  def S : Subst T F := λ n => HasVar.to (n + 1)
-  -- def Sn (k : Nat) : Subst T := λ n => #(n + k)
+  def Subst.id : Subst T := λ n => .re n
+  def Subst.succ : Subst T := λ n => .re (n + 1)
 
-  @[simp] theorem I_action {n} : I n = HasVar.to (T := F T) n := by unfold I; simp
+  notation "+0" => Subst.id
+  notation "+1" => Subst.succ
 
-  @[simp] theorem S_action {n} : S n = HasVar.to (T := F T) (n + 1) := by unfold S; simp
-  -- @[simp] theorem Sn_action {k n} : @Sn T k n = #(n + k) := by unfold Sn; simp
-
-  @[simp]
-  theorem to_I : Ren.to (λ x => x) = I (T := T) (F := F) := by
-    unfold Ren.to; simp; unfold I; simp
+  theorem Subst.id_action {n} : @Subst.id T n = .re n := by simp [Subst.id]
+  theorem Subst.succ_action {n} : @Subst.succ T n = .re (n + 1) := by simp [Subst.succ]
 
   @[simp]
-  theorem to_S : Ren.to (λ x => x + 1) = S (T := T) (F := F) := by
-    unfold Ren.to; simp; unfold S; simp
+  theorem Ren.to_id : Ren.to (λ x => x) = @Subst.id T := by
+    unfold Ren.to; unfold Subst.id; simp
 
-  -- @[simp]
-  -- theorem to_Sn {k} : Ren.to (λ x => x + k) = @Sn T k := by
-  --   unfold Ren.to; simp; unfold Sn; simp
+  @[simp]
+  theorem Ren.to_succ : Ren.to (λ x => x + 1) = @Subst.succ T := by
+    unfold Ren.to; simp; unfold Subst.succ; simp
 
   macro:max t:term noWs "[" σ:term "]" : term => `(Subst.apply $σ $t)
---  notation t "[" σ "]" => Subst.apply σ t
   infixr:85 " ∘ " => Subst.compose
 
-  def test (xs : List Nat) (y : Nat) (h : y < xs.length) : Nat := xs[y]
+  class SubstMapStable (T : Type) [SubstMap T] where
+    apply_id {t : T} : t[+0] = t
+    apply_stable (r : Ren) (σ : Subst T) : r = σ -> Ren.apply r = Subst.apply σ
 
-  class SubstMapStable (T : Type u) (F : Type u -> Type u) [HasVar T] [Monad F] [ActionOps T F] [LawfulMonad F] [SubstMap T F] where
-    apply_id {t : T} : t[I (T := T) (F := F)] = t
-    apply_stable {r} {σ : Subst T F} : r.to = σ -> Ren.apply (T := T) (F := F) r = Subst.apply σ
+  class SubstMapCompose (T : Type) [SubstMap T] where
+    apply_compose {s : T} {σ τ : Subst T} : s[σ][τ] = s[σ ∘ τ]
 
-  class SubstMapCompose (T : Type u) (F : Type u -> Type u) [HasVar T] [Monad F] [ActionOps T F] [LawfulMonad F] [SubstMap T F] where
-    apply_compose {s : T} {σ τ : Subst T F} : s[σ][τ] = s[σ ∘ τ]
+  theorem Ren.lift_to_commute [SubstMap T] {r : Ren} : r.lift.to = (@Ren.to T r).lift := by
+    funext; case _ x =>
+    cases x
+    case zero =>
+      unfold Ren.to; unfold Ren.lift; simp
+      unfold Subst.lift; simp
+    case _ n =>
+      generalize lhsdef : ((@Ren.to T r.lift)) (n + 1) = lhs
+      generalize rhsdef : ((@Ren.to T r).lift) (n + 1) = rhs
+      unfold Ren.to at lhsdef; simp [Ren.to] at *
+      unfold Ren.lift at lhsdef; simp at *
+      unfold Subst.lift at rhsdef; simp at *
+      subst lhsdef; subst rhsdef; rfl
 
-  namespace Ren
-    section
-      variable [LawfulMonad F] [SubstMap T F] [SubstMapVar T F]
-
-      theorem lift_to_commute {r : Ren} : r.lift.to = (Ren.to (T := T) (F := F) r).lift := by
-        funext; case _ x =>
-        cases x
-        case zero =>
-          unfold Ren.to; unfold Ren.lift; simp
-          unfold Subst.lift; simp
-        case _ n =>
-          generalize lhsdef : ((Ren.to (T := T) (F := F) r.lift)) (n + 1) = lhs
-          generalize rhsdef : ((Ren.to (T := T) (F := F) r).lift) (n + 1) = rhs
-          unfold Ren.to at lhsdef; simp at *
-          unfold Ren.lift at lhsdef; simp at *
-          unfold Subst.lift at rhsdef; simp at *
-          subst lhsdef; subst rhsdef
-          unfold apply; simp [Ren.to]
-    end
-  end Ren
+  theorem Ren.lift_eq_from_eq [SubstMap T] {r : Ren} {σ : Subst T} : r = σ -> r.lift = σ.lift := by
+    intro h; rw [<-h, lift_to_commute]
 
   namespace Subst
     section
       @[simp] -- 0.S = I
-      theorem rewrite1 : HasVar.to 0 :: S = I (T := T) (F := F) := by
+      theorem rewrite1 : .re 0 :: +1 = @Subst.id T := by
         funext; case _ x =>
-        cases x; all_goals (unfold Sequence.cons; unfold S; unfold I; simp)
+        cases x; all_goals (simp [Sequence.cons, Subst.id, Subst.succ])
 
-      variable [LawfulMonad F] [SubstMap T F] [SubstMapVar T F]
+      variable [SubstMap T]
       open SubstMap
 
       @[simp]
-      theorem I_lift : I.lift = I (T := T) (F := F) := by
+      theorem I_lift : +0.lift = @Subst.id T := by
         funext; case _ x =>
-        cases x; all_goals (simp [Subst.lift, I, Ren.apply])
+        cases x; all_goals (simp [Subst.lift, Subst.id])
 
       @[simp] -- σ ◦ I = σ
-      theorem rewrite2 {σ : Subst T F} : I ∘ σ = σ := by
+      theorem rewrite2 {σ : Subst T} : +0 ∘ σ = σ := by
         funext; case _ x =>
-        unfold Subst.compose; unfold I; simp [Subst.apply]
+        unfold Subst.compose; simp [Subst.id]
 
       @[simp] -- (s.σ ) ◦ τ = s[τ].(σ ◦ τ)
-      theorem rewrite3_replace {σ τ : Subst T F} {s : T}
-        : (pure s :: σ) ∘ τ = pure s[τ] :: (σ ∘ τ)
+      theorem rewrite3_replace {σ τ : Subst T} {s : T}
+        : (.su s :: σ) ∘ τ = .su s[τ] :: (σ ∘ τ)
       := by
         funext; case _ x =>
-        cases x; all_goals (simp [Subst.compose, Sequence.cons, Subst.apply])
-        unfold Function.comp; simp; congr
-        funext; case _ f x =>
-        cases x <;> simp [Subst.lift, Ren.apply]
-        sorry -- probably true?
+        cases x; all_goals (simp [Subst.compose, Sequence.cons])
 
       @[simp] -- (s.σ ) ◦ τ = s[τ].(σ ◦ τ)
       theorem rewrite3_rename {s} {σ τ : Subst T}
-        : (#s :: σ) ∘ τ = (τ s) :: (σ ∘ τ)
+        : (.re s :: σ) ∘ τ = (τ s) :: (σ ∘ τ)
       := by
         funext; case _ x =>
         cases x; all_goals (simp [Subst.compose, Sequence.cons])
 
       @[simp] -- S ◦ (s.σ ) = σ
-      theorem rewrite4 {s} {σ : Subst T} : S ∘ (s :: σ) = σ := by
+      theorem rewrite4 {s} {σ : Subst T} : +1 ∘ (s :: σ) = σ := by
         funext; case _ x =>
-        cases x; all_goals (simp [Subst.compose, Sequence.cons, S])
+        cases x; all_goals (simp [Subst.compose, Sequence.cons, Subst.succ])
 
       @[simp] -- 0[σ ].(S ◦ σ ) = σ
-      theorem rewrite5 {σ : Subst T} : σ 0 :: (S ∘ σ) = σ := by
+      theorem rewrite5 {σ : Subst T} : σ 0 :: (+1 ∘ σ) = σ := by
         funext; case _ x =>
         cases x
         case _ => simp
-        case _ => simp [S, Subst.compose]
+        case _ => simp [Subst.succ, Subst.compose]
 
       variable [SubstMapStable T]
       open SubstMapStable
 
       @[simp]
-      theorem apply_I_is_id {s : T} : s[I] = s :=
+      theorem apply_I_is_id {s : T} : s[+0] = s :=
         SubstMapStable.apply_id
 
       @[simp] -- ⇑σ = 0.(σ ◦ S)
-      theorem rewrite_lift {σ : Subst T} : σ.lift = #0 :: (σ ∘ S) := by
+      theorem rewrite_lift {σ : Subst T} : σ.lift = .re 0 :: (σ ∘ +1) := by
         funext; case _ x =>
         cases x
         case _ => simp [Subst.lift]
         case _ n =>
-          simp [Subst.lift, S, Subst.compose]
+          simp [Subst.lift, Subst.succ, Subst.compose]
           generalize tdef : σ n = t
           cases t <;> simp at *
           case _ y =>
             rw [apply_stable]
-            funext; case _ i => simp [Ren.to]
+            funext; case _ i => simp [Ren.to, Subst.succ]
 
       @[simp] -- I ◦ σ = σ
-      theorem rewrite6 {σ : Subst T} : σ ∘ I = σ := by
+      theorem rewrite6 {σ : Subst T} : σ ∘ +0 = σ := by
         funext; case _ x =>
-        unfold Subst.compose; unfold I; unfold Subst.apply; simp
+        simp [Subst.compose, Subst.id, Subst.apply]
         generalize zdef : σ x = z
-        cases z <;> simp at *
-        have lem : smap Subst.lift (λ x => #x) = @Subst.apply T _ I := by
-          unfold Subst.apply; unfold I; simp
-        rw [lem, apply_id]
+        cases z <;> simp at *; case _ t =>
+        have lem := apply_id (T := T) (t := t)
+        simp [Subst.apply] at lem; exact lem
     end
 
     section
@@ -250,81 +196,69 @@ namespace LeanSubst
       @[simp] -- (σ ◦ τ) ◦ μ = σ ◦ (τ ◦ μ)
       theorem rewrite7 {σ τ μ : Subst T} : (σ ∘ τ) ∘ μ = σ ∘ τ ∘ μ := by
         funext; case _ x =>
-        unfold Subst.compose; simp
+        simp [Subst.compose]
         cases σ x <;> simp
-        . unfold Subst.compose; simp
     end
   end Subst
 
   macro "solve_stable" r:term "," σ:term : tactic => `(tactic| {
-    intro h; funext; case _ x =>
-    unfold Ren.apply; simp [SubstMap.smap] at *
-    unfold Ren.to; simp
-    induction x generalizing $r $σ <;> simp at *
-    any_goals simp [*]
-    case _ x => rw [<-h]; unfold Ren.to; simp
-    all_goals
-      rw [Ren.lift_to_commute, <-h]
-      unfold Ren.fro; simp
+    intro h; simp [Ren.apply, Subst.apply]
+    funext; case _ t =>
+    induction t generalizing $r $σ <;> simp [Ren.to] at *
+    all_goals simp [SubstMap.smap, *] at *; try simp [*]
+    any_goals solve | (
+      rw [<-Ren.lift_eq_from_eq h]
+      simp [Ren.to])
+    any_goals solve | (rw [<-h]; simp)
   })
 
   macro "solve_compose" Ty:term "," s:Lean.Parser.Tactic.elimTarget "," σ:term "," τ:term : tactic => `(tactic| {
     have lem1 (τ : Subst $Ty) : (Ren.to (· + 1)) ∘ τ.lift = τ ∘ (Ren.to (· + 1)) := by
       funext; case _ x =>
       cases x <;> simp
-    have lem1s (τ : Subst $Ty) : S ∘ τ.lift = τ ∘ S := by
-      rw [<-to_S, lem1]
-    have lem2 {σ : Subst $Ty} {r} : ((Ren.to r) ∘ σ).lift = (Ren.to r).lift ∘ σ.lift := by
+    have lem1s (τ : Subst $Ty) : +1 ∘ τ.lift = τ ∘ +1 := by
       funext; case _ x =>
       cases x <;> simp
-      case _ x =>
-        simp [Ren.to, Subst.compose]
-    have lem2s {σ : Subst $Ty} : (S ∘ σ).lift = S.lift ∘ σ.lift := by
-      rw [<-to_S, lem2]
-    have lem3 {σ : Subst $Ty} {r t} : t[Ren.to r][σ] = t[(Ren.to r) ∘ σ] := by
-      induction t generalizing σ r
-      all_goals simp [-Subst.rewrite_lift, *]
-      all_goals try rw [<-Ren.lift_to_commute]; simp [*]
-      all_goals try (
-        simp [Subst.compose]
-        split <;> simp [*]
-      )
-    have lem3s {σ : Subst $Ty} {t} : t[S][σ] = t[S ∘ σ] := by
-      rw [<-to_S, lem3]
-    have lem4 {σ τ : Subst $Ty} : S ∘ τ ∘ σ = (S ∘ τ) ∘ σ := by
+    have lem2 {σ : Subst $Ty} {r} : (r ∘ σ).lift = (Ren.to r).lift ∘ σ.lift := by
       funext; case _ x =>
-      cases x <;> simp [Subst.compose]
-    have lem5 {r1 r2} {τ : Subst $Ty}
-      : (τ ∘ (Ren.to r2)) ∘ Ren.to r1 = τ ∘ (Ren.to r2) ∘ Ren.to r1
-    := by
+      cases x <;> simp
+      case _ x => simp [Ren.to, Subst.succ, Subst.compose]
+    have lem2s {σ : Subst $Ty} : (+1 ∘ σ).lift = +1.lift ∘ σ.lift := by rw [<-Ren.to_succ, lem2]
+    have lem3 {σ : Subst $Ty} {r : Ren} {t} : t[r][σ] = t[r ∘ σ] := by
+      induction t generalizing σ r
+      any_goals solve | simp [*]
+      any_goals solve | (
+        simp [-Subst.rewrite_lift, *]
+        rw [<-Ren.lift_to_commute]; simp [*])
+    have lem3s {σ : Subst $Ty} {t} : t[+1][σ] = t[+1 ∘ σ] := by rw [<-Ren.to_succ, lem3]
+    have lem4 {σ τ : Subst $Ty} : +1 ∘ τ ∘ σ = (+1 ∘ τ) ∘ σ := by
+      funext; case _ x =>
+      cases x <;> simp [Subst.compose, Subst.succ]
+    have lem5 {r1 r2 : Ren} {τ : Subst $Ty} : (τ ∘ r2.to) ∘ r1.to = τ ∘ r2.to ∘ r1.to := by
       funext; case _ x =>
       unfold Subst.compose; simp
       cases τ x <;> simp [*]
       unfold Subst.compose; simp
-    have lem6 {τ : Subst $Ty} {r} : (τ ∘ (Ren.to r)).lift = τ.lift ∘ (Ren.to r).lift := by
+    have lem6 {τ : Subst $Ty} {r : Ren} : (τ ∘ r.to).lift = τ.lift ∘ r.to.lift := by
       funext; case _ x =>
       cases x; simp
       case _ x =>
         simp [Subst.compose]
-        cases τ x <;> simp [*]
-    have lem6s {τ : Subst $Ty} : (τ ∘ S).lift = τ.lift ∘ S.lift := by
-      rw [<-to_S, lem6]
-    have lem7 {τ : Subst $Ty} {t r} : t[τ][Ren.to r] = t[τ ∘ (Ren.to r)] := by
+        cases τ x <;> simp [Subst.succ, *]
+    have lem6s {τ : Subst $Ty} : (τ ∘ +1).lift = τ.lift ∘ +1.lift := by rw [<-Ren.to_succ, lem6]
+    have lem7 {τ : Subst $Ty} {t} {r : Ren} : t[τ][r] = t[τ ∘ r.to] := by
       induction t generalizing τ r
-      all_goals simp [-Subst.rewrite_lift, *]
-      all_goals try rw [<-Ren.lift_to_commute]; simp [*]
-      all_goals try (
-        simp [Subst.compose]
-        split <;> simp [*]
-      )
-    have lem7s {τ : Subst $Ty} {t} : t[τ][S] = t[τ ∘ S] := by
-      rw [<-to_S, lem7]
-    have lem8 {σ τ : Subst $Ty} : (σ ∘ S) ∘ τ = σ ∘ S ∘ τ := by
+      any_goals solve | simp [*]
+      any_goals solve | (
+        simp [-Subst.rewrite_lift, *]
+        rw [<-Ren.lift_to_commute]; simp [*])
+    have lem7s {τ : Subst $Ty} {t} : t[τ][+1] = t[τ ∘ +1] := by rw [<-Ren.to_succ, lem7]
+    have lem8 {σ τ : Subst $Ty} : (σ ∘ +1) ∘ τ = σ ∘ +1 ∘ τ := by
       funext; case _ x =>
       unfold Subst.compose; simp
       cases σ x <;> simp at *
       rw [lem3s]; unfold Subst.compose; simp
-    have lem9 {σ τ : Subst $Ty} : ((σ ∘ τ) ∘ S) = σ ∘ τ ∘ S := by
+    have lem9 {σ τ : Subst $Ty} : ((σ ∘ τ) ∘ +1) = σ ∘ τ ∘ +1 := by
       funext; case _ x =>
       unfold Subst.compose; simp
       cases σ x <;> simp at *
@@ -333,12 +267,10 @@ namespace LeanSubst
       funext; case _ x =>
       cases x <;> simp [*]
     induction $s generalizing $σ $τ
-    all_goals simp [-Subst.rewrite_lift, *]
-    all_goals try rw [<-Ren.lift_to_commute]; simp [*]
-    all_goals try (
-      simp [Subst.compose]
-      split <;> simp [*]
-    )
+    any_goals solve | simp [*]
+    try any_goals solve | (
+      simp [-Subst.rewrite_lift, *]
+      rw [<-Ren.lift_to_commute]; simp [*])
   })
 
 end LeanSubst
