LeanSubst.lean
@@ -1,10 +1,8 @@
 -- This module serves as the root of the `LeanSubst` library.
 -- Import modules here that should be built as part of the library.
-import LeanSubst.Notation
 import LeanSubst.Basic
 import LeanSubst.Map
 import LeanSubst.Reduction
 import LeanSubst.Normal
 import LeanSubst.Subtype
 import LeanSubst.Coe
-import LeanSubst.IsRen
