LeanSubst/Map.lean
@@ -2,8 +2,7 @@ import LeanSubst.Basic
 
 namespace LeanSubst.Subst
   section
-    universe u v
-    variable {A : Type u} {B : Type v} {f : A -> B}
+    variable {A : Type} {B : Type} {f : A -> B}
 
     @[simp]
     def map {A B} (f : A -> B) : Subst A -> Subst B
@@ -13,12 +12,12 @@ namespace LeanSubst.Subst
       | .re k => .re k
 
     @[simp]
-    theorem map_rename_seq {k} {σ : Subst A} : map f (#k :: σ) = #k :: map f σ := by
+    theorem map_rename_seq {k} {σ : Subst A} : map f (.re k :: σ) = .re k :: map f σ := by
       funext; case _ x =>
       cases x <;> simp
 
     @[simp]
-    theorem map_replace_seq {t} {σ : Subst A} : map f (%t :: σ) = %(f t) :: map f σ := by
+    theorem map_replace_seq {t} {σ : Subst A} : map f (.su t :: σ) = .su (f t) :: map f σ := by
       funext; case _ x =>
       cases x <;> simp
 
@@ -29,10 +28,10 @@ namespace LeanSubst.Subst
       cases x <;> simp
 
     @[simp]
-    theorem map_I_noop : map f I = I := by apply map_rename_noop
+    theorem map_I_noop : map f +0 = +0 := by apply map_rename_noop
 
     @[simp]
-    theorem map_S_noop : map f S = S := by apply map_rename_noop
+    theorem map_S_noop : map f +1 = +1 := by apply map_rename_noop
 
     theorem map_rename_compose_left {τ : Subst A} [SubstMap A] [SubstMap B] {f : A -> B} {r : Ren}
       : (∀ t, f t[r.to] = (f t)[r.to]) -> map f (τ ∘ r.to) = (map f τ) ∘ r.to
@@ -54,14 +53,14 @@ namespace LeanSubst.Subst
         unfold Ren.to; simp
 
     theorem map_S_compose_left {τ : Subst A} [SubstMap A] [SubstMap B] {f : A -> B}
-      : (∀ t, f t[S] = (f t)[S]) -> map f (τ ∘ S) = (map f τ) ∘ S
+      : (∀ t, f t[+1] = (f t)[+1]) -> map f (τ ∘ +1) = (map f τ) ∘ +1
     := by
       intro h
       apply map_rename_compose_left h
 
     @[simp]
     theorem map_S_compose_right {σ : Subst A} [SubstMap A] [SubstMap B] {f : A -> B}
-      : map f (S ∘ σ) = S ∘ (map f σ)
+      : map f (+1 ∘ σ) = +1 ∘ (map f σ)
     := by apply map_rename_compose_right
   end
 end LeanSubst.Subst
